restructuring of files and modules and added a main method

ServiceProvider.fst
@@ -1,11 +1,19 @@
-module ILIST1
+module SERVICEPROVIDER
+open PROTOCOL
 
-type ilist :: int => * => * = 
-   | INil  : ilist 0 'a
-   | ICons : x:'a -> n:int -> ilist n 'a -> ilist (n + 1) 'a
+(*
+- Protocol events
+- Add assumtions
+- Add asserts
+*)
 
-val iappend: n1:int -> ilist n1 'a -> n2:int -> ilist n2 'a -> ilist (n1 + n2) 'a
-let rec iappend n1 l1 n2 l2 = match l1 with
-   | INil -> l2
-   | ICons x n1_minus_1 l1tl ->
-     ICons x (n1_minus_1 + n2) (iappend n1_minus_1 l1tl n2 l2)
+val serviceprovider: me:prin -> client:prin -> idp:prin -> unit 
+let serviceprovider me client idp = 
+  let reqUri = recieveHttpRequest client in (*1*)
+    let (authnReq, sigSP)  = createAuthnRequest me idp in 
+      sendAuthnRequest client authnReq sigSP "relay"; (*2*)
+      let (sp, samlResponse, sigIDP, relay) = recievehttpRedirect client in (*7*)
+        sendResource client; (*8*)
+        ()
+
+end (* SERVICEPROVIDER *)
