SimpleCrypto.fst
@@ -36,12 +36,14 @@ open UTIL
 val client: me:prin -> pubkey me -> privkey me 
          -> server:prin -> pubkey server -> unit
 let client me mypk mysk server serverpk = 
-   let req = string2bytes "Hi server" in assume (Says me req); (* protocol event *)
-   let dsig = sign me mysk req in send server (req, dsig);
-   let (resp, dsig') = recv server in 
-    if verify server serverpk resp dsig'
-    then (assert (Says server resp); ())
-    else ()
+   let req = string2bytes "Hi server" in 
+    assume (Says me req); (* protocol event *)
+    let dsig = sign me mysk req in 
+      send server (req, dsig);
+      let (resp, dsig') = recv server in 
+        if verify server serverpk resp dsig'
+        then (assert (Says server resp); ())
+        else ()
 
 end(* client *)
 
