client.fst
@@ -1,0 +1,21 @@
+module CLIENT
+open PROTOCOL
+
+(*
+- Protocol events
+- Add assumtions
+- Add asserts
+  *)
+
+val client: me:prin -> user:string -> password:string -> unit
+let client sp user password = 
+    let _ = sendRequestResource sp in(*1*)
+      let (idp, authnRequest, sigSP, relayState) = recievehttpRedirect sp in(*2*)
+        sendAuthnRequest idp authnRequest sigSP relayState;(*3*)
+        let challenge = recieveAutenticationRequestChallenge idp in(*4*)
+          sendAutenticationRequest idp user password challenge; (*5*)
+          let (sp', samlResponse, sigIDP, relayState') = recievehttpRedirect idp in(*6*)
+            sendAuthentication sp' samlResponse relayState'; (*7*)
+            let res = recieveHttpResponse sp' in (*8*)
+            ()
+end (*CLIENT*)
