identityprovider.fst
@@ -1,0 +1,20 @@
+module IDENTITYPROVIDER
+open PROTOCOL
+
+(*
+- Protocol events
+- Add assumtions
+- Add asserts
+*)
+
+val identityprovider: me:prin -> client:prin -> sp:prin -> unit
+let identityprovider me client serviceprovider =
+  let (authnReq, sigSP, relay) = recieveAutenticationRequest client in (*3*)
+    let challenge = createChallenge client in
+      sendAutenticationChallenge client challenge; (*4*)
+      let (user,password, challenge') = recieveAutenticationCredentials client in (*5*)
+        let (samlResponse, sigIDP) = createSamlResponse me serviceprovider in 
+          sendhttpRedirect client serviceprovider samlResponse sigIDP; (*6*)
+          ()
+
+end (*IDENTITYPROVIDER*)
