main.fst
@@ -1,0 +1,8 @@
+module MAIN
+open PROTOCOL
+open CLIENT
+
+val main: sp:prin -> user:string -> password:string -> unit
+let main sp user password = 
+	client sp user password
+end
